theories/interop/wrapper_wp_simulation.v
@@ -1,0 +1,165 @@
+From Coq Require Import ssreflect.
+From stdpp Require Import strings gmap.
+From melocoton.mlanguage Require Import mlanguage.
+From melocoton.language Require Import language weakestpre.
+From melocoton.mlanguage Require Import weakestpre.
+From melocoton.interop Require Import wrappersem wrapperstate.
+From iris.base_logic.lib Require Import ghost_map ghost_var gset_bij.
+From iris.algebra Require Import gset gset_bij.
+From melocoton Require Import big_sepM_limited.
+From iris.proofmode Require Import proofmode.
+From melocoton.c_toy_lang Require Import lang melocoton.lang_instantiation melocoton.primitive_laws.
+From melocoton.ml_toy_lang Require Import lang melocoton.lang_instantiation melocoton.primitive_laws.
+From melocoton.interop Require Import linking_wp basics wrapper_wp wrapper_wp_block_sim.
+Import Wrap.
+
+Section Simulation.
+
+Context {hlc : has_lc}.
+Context {Σ : gFunctors}.
+Context `{!heapGS_ML Σ, !heapGS_C Σ}.
+Context `{!invGS_gen hlc Σ}.
+Context `{!wrapperGS Σ}.
+
+Notation MLval := ML_lang.val.
+Notation Cval := C_lang.val.
+
+Implicit Types P : iProp Σ.
+Import mlanguage.
+
+
+Notation mkPeC p T := ({| penv_prog := p; penv_proto := T |} : prog_environ _ Σ).
+Notation mkPeW p T := ({| weakestpre.penv_prog := p; weakestpre.penv_proto := T |} : weakestpre.prog_environ wrap_lang Σ).
+
+
+Definition WP_ext_call_spec : string -d> list Cval -d> (Cval -d> iPropO Σ) -d> iPropO Σ := λ n vl wp,
+  ⌜False⌝%I.
+
+Definition forbidden_function_names : list string := ["alloc"; "registerroot"; "unregisterroot"; "modify"; "readfield"; "int2val"; "val2int"].
+
+Notation wrap_return := (fun Φ (a:Cval) => (∃ θ' l v, GC θ' ∗ Φ v ∗ ⌜repr_lval θ' l a⌝ ∗ block_sim v l)%I).
+
+
+Lemma wp_to_val E p T a Φ: 
+    wrap_return Φ a
+ -∗ not_at_boundary
+ -∗ WP (ExprC (C_lang.Val a)) @ (mkPeW (p : prog wrap_lang) T); E {{ v, Φ v ∗ at_boundary _}}.
+Proof.
+  iIntros "(%θ & %l & %v & HGC & Hv & %Hrepr & #Hblock) Hnb".
+  rewrite weakestpre.wp_unfold. rewrite /weakestpre.wp_pre.
+  iIntros "%σ Hσ".
+  iDestruct (GC_in_C with "Hσ HGC") as "%H"; destruct H as (ρc & mem & ->).
+  iDestruct "Hσ" as SIC_ip.
+  iDestruct "HGC" as GC_ip.
+  iRight. iRight. iModIntro. iSplit.
+  1: iPureIntro; cbn; exists (fun _ => True); eexists (), _; repeat split; by eapply RetS.
+  cbn. iIntros (X Hstep).
+  destruct Hstep as ([] & e1 & Heq & Hstep).
+  cbv in Heq; subst e1.
+  inversion Hstep.
+  1: exfalso; apply language.language.val_stuck in H3; cbn in H3; done.
+  2-8: exfalso; unfold language.to_call in H2; destruct language.to_class as [[]|] eqn:Heq; try congruence;
+       destruct (language.fill_class' K ec) as [?|[vv ?]];
+       [exists (ExprVal a); cbn; by rewrite H
+       |subst K; cbn in *; subst ec; cbn in Heq; congruence| congruence].
+  cbn in H3; injection H3; intros <-.
+  iAssert (⌜is_val χvirt ζfreeze v l⌝)%I as "%Hval".
+  1: iApply (block_sim_to_ghost_state with "HAχbij HAζbl"); done.
+
+  iPoseProof (ghost_var_agree with "HAGCθ HAθ") as "->".
+  iPoseProof (ghost_var_agree with "HArootss HAroots") as "->".
+  iPoseProof (@fractional.fractional_merge _ (ghost_var wrapperGS_γat_boundary (1 / 4) false) (ghost_var wrapperGS_γat_boundary (1 / 4) false) _ (1/4) (1/4) (ghost_var_fractional _ _) with "HAGCbound HAbound") as "Hnb'".
+  assert ((1 / 4 + 1 / 4 = 1 / 2)%Qp) as -> by compute_done.
+  iMod (ghost_var_update_halves with "Hnb Hnb'") as "(Hnb & Hbound)".
+
+  do 3 iModIntro. do 2 iExists _.  iSplit.
+  1: iPureIntro; eapply (H4 σMLvirt l v ζfreeze ζσ χvirt ζrest roots_m mem).
+  all: try done.
+  1: rewrite map_union_comm; done.
+  1: apply map_disjoint_dom_1; eapply map_disjoint_spec; intros ?????; by eapply map_disjoint_spec.
+  1: admit.
+  iSplitR "Hv Hnb"; last first.
+  1: { cbn. unfold Wrap.fill. iApply weakestpre.wp_value'. iFrame. }
+  cbn. iSplitL "HAσMLv HAnMLv".
+  1: iExists nMLv; iFrame.
+  unfold private_state_interp, ML_state_interp; cbn.
+Admitted.
+
+Lemma wp_simulates E p T ec Φ: 
+    ⌜Forall (fun k => p !! k = None) forbidden_function_names⌝
+ -∗ not_at_boundary
+ -∗ WP ec @ (mkPeC p WP_ext_call_spec); E {{a, wrap_return Φ a }}
+ -∗ WP (ExprC ec) @ (mkPeW (p : prog wrap_lang) T); E {{ v, Φ v ∗ at_boundary _}}.
+Proof.
+  iIntros "%Hforbid".
+  iLöb as "IH" forall (ec).
+  rewrite weakestpre.wp_unfold. rewrite /weakestpre.wp_pre.
+  rewrite wp_unfold. rewrite /wp_pre.
+  iIntros "Hnb HWP %σ Hσ".
+  destruct σ as [ρml σ | ρc mem].
+  1: iExFalso; iClear "HWP"; iDestruct "Hσ" as SIML_ip; iPoseProof (ghost_var_agree with "Hnb HAbound") as "%HH"; congruence.
+  iDestruct "Hσ" as SIC_ip.
+  iMod ("HWP" $! mem nCv with "HσC") as 
+  "[(%x & -> & Hσ & Hret)
+  |[(%s' & %vv & %K' & -> & %H2 & >(%Ξ & Hσ & HT & Hr))
+  |(%Hred & H3)]]".
+  + iPoseProof (wp_to_val with "Hret") as "Hret".
+    iSpecialize ("Hret" with "Hnb").
+    rewrite weakestpre.wp_unfold. rewrite /weakestpre.wp_pre.
+    iApply ("Hret" $! (CState ρc mem)).
+    iSplitL "Hσ". 1: by iExists _.
+    unfold C_state_interp.
+    iExists ζfreeze, ζσ, ζrest, χvirt, fresh, σMLvirt.
+    iFrame. iFrame "HAζpers".
+    iSplitL "HAnMLv"; first by iExists nMLv.
+    iPureIntro. split_and!; done.
+  + cbn. iExFalso. iApply "HT". (* TODO: add more calls here *)
+  + cbn in Hred. iModIntro. iRight. iRight. iSplit.
+    * iPureIntro. exists (fun _ => True). eapply head_prim_step.
+      destruct Hred as (e' & σ' & Hprim). econstructor; last done. cbn. eapply Hprim.
+    * iIntros (X Hstep).
+      destruct Hstep as ([] & x & Hre & Hstep). cbv in Hre; subst x.
+      cbn in Hstep; unfold step,mrel in Hstep; cbn in Hstep.
+      inversion Hstep. 2-9: exfalso.
+      2: { apply C_lang.of_to_val in H3; subst ec.
+           apply language.language.reducible_no_threads_reducible in Hred.
+           apply language.language.reducible_not_val in Hred. cbn in Hred; congruence. }
+      2-8: subst ec; eapply reducible_call_is_in_prog; 
+           [ by eapply language.language.reducible_no_threads_reducible
+           | done
+           | eapply @List.Forall_forall in Hforbid; [apply Hforbid | cbv; eauto 20]].
+      subst ec0 ρc0 mem0 X0. cbn.
+      iMod ("H3" $! _ _ H3) as "H3".
+      do 2 iModIntro. iMod "H3" as "(HσC & HWP')".
+      iModIntro. iExists _, _. iSplitR; first (iPureIntro; apply H4).
+      iSplitR "HWP' Hnb".
+      2: iApply ("IH" with "Hnb HWP'").
+      cbn. iSplitL "HσC"; first by iExists _.
+      unfold C_state_interp. iExists ζfreeze, ζσ, ζrest, χvirt, fresh, σMLvirt.
+      iFrame. iFrame "HAζpers". iSplitL; first by iExists _.
+      iPureIntro; split_and!; done.
+Qed.
+
+
+Lemma run_function_correct F (vv : list ML_lang.val) T p E Φ: 
+    ⌜arity F = length vv⌝
+ -∗ at_boundary _
+ -∗ (∀ θ ll aa ec, 
+       GC θ 
+    -∗ ⌜C_lang.apply_function F aa = Some ec⌝
+    -∗ ([∗ list] l;a ∈ ll;aa, ⌜repr_lval θ l a⌝)
+    -∗ block_sim_arr vv ll
+    -∗ WP ec @ (mkPeC p WP_ext_call_spec); E {{a, wrap_return Φ a }})
+ -∗ WP RunFunction F vv @ (mkPeW (p : prog wrap_lang) T); E {{ v, Φ v ∗ at_boundary _}}.
+Proof.
+  iIntros "%Harity Hb Hwp".
+  rewrite weakestpre.wp_unfold. rewrite /weakestpre.wp_pre.
+  iIntros (σ) "Hσ".
+  unfold at_boundary; cbn. destruct σ as [ρml σ | ? ?].
+  2: {iExFalso. iDestruct "Hσ" as SIC_ip. iPoseProof (ghost_var_agree with "Hb HAbound") as "%Heq". congruence. }
+  iRight. iRight. iModIntro.
+  iSplitR.
+  1: { iPureIntro. exists (fun _ => True). eapply mlanguage.head_prim_step. cbn. eapply RunFunctionS; last done. all: admit. }
+Admitted.
+
+End Simulation.
